src/program_proof/mvcc/txn_commit.v
@@ -3,8 +3,14 @@ From Perennial.program_proof.mvcc Require Import txn_common.
 Section program.
 Context `{!heapGS Σ, !mvcc_ghostG Σ}.
 
+Definition abort_cases γ : iProp Σ :=
+  (∃ tid, nca_tids_frag γ tid) ∨
+  (∃ tid, fa_tids_frag γ tid)  ∨
+  (∃ tmod, fci_tmods_frag γ tmod) ∨
+  (∃ tmod, fcc_tmods_frag γ tmod).
+
 Theorem wp_txn__Commit_false txn tid γ τ :
-  {{{ own_txn_ready txn tid γ τ }}}
+  {{{ own_txn_ready txn tid γ τ ∗ abort_cases γ }}}
     Txn__Commit #txn
   {{{ (ok : bool), RET #ok; False }}}.
 Admitted.
